Analysis/exercises/Nelson-ch0-defs.dfy
@@ -1,0 +1,196 @@
+include "../definitions.dfy"
+
+module NelsonCh0Defs {
+    import opened Analysis
+
+    predicate boundedOutput(f: real --> real, x: real, M: real)
+        requires f.requires(x)
+    {
+        abs(f(x)) <= M
+    }
+
+    ghost predicate isBoundedBetween(f: real --> real, a: real, b: real, M: real)
+        requires M > 0.0
+    {
+        forall x: real :: a <= x <= b ==> if f.requires(x) then boundedOutput(f, x, M) else false
+    }
+
+    ghost predicate isBounded(f: real --> real, a: real, b: real) {
+        exists M: real :: M > 0.0 && isBoundedBetween(f, a, b, M)
+    }
+
+    lemma functionBoundedInMiddle(f: real --> real, a: real, b: real, c: real)
+        requires a < c < b
+        requires isBounded(f, a, b)
+        ensures isBounded(f, a, c)
+        ensures isBounded(f, c, b)
+    {
+        var M :| M > 0.0 && isBoundedBetween(f, a, b, M);
+        assert isBoundedBetween(f, a, c, M);
+        assert isBoundedBetween(f, c, b, M);
+    }
+
+    ghost function BoundedFunctions(a: real, b: real): iset<real -> real> 
+        requires a <= b
+    {
+        iset f: real -> real | isBounded(f, a, b)
+    }
+
+    lemma BoundedFunctionsSubset(a: real, b: real, c: real, f: real -> real)
+        requires a < c < b
+        requires isBounded(f, a, b)
+        ensures isBounded(f, c, b)
+    {
+        var M :| M > 0.0 && isBoundedBetween(f, a, b, M);
+        assert isBoundedBetween(f, c, b, M);
+    }
+
+    lemma BoundedFunctionsSubsetLower(a: real, b: real, c: real, f: real -> real)
+        requires a < c < b
+        requires isBounded(f, a, b)
+        ensures isBounded(f, a, c)
+    {
+        var M :| M > 0.0 && isBoundedBetween(f, a, b, M);
+        assert isBoundedBetween(f, a, c, M);
+    }
+
+    ghost function funcRange(f: real --> real, a: real, b: real): iset<real>
+        requires forall x :: a <= x <= b ==> f.requires(x)
+    {
+        iset x | a <= x <= b :: f(x)
+    }
+
+    ghost function infimum(ms: iset<real>, val: real, lbound: real): real
+        requires val in ms
+        requires lowerBound(ms, lbound)
+        ensures inf(ms, infimum(ms, val, lbound))
+    {
+        CompletenessAxiomLower(ms, lbound);
+        var inf_ms :| inf(ms, inf_ms);
+        inf_ms
+    }
+
+    lemma infimumUnique(ms: iset<real>, val: real, val': real, bound: real, bound': real)
+        requires val in ms
+        requires val' in ms
+        requires lowerBound(ms, bound)
+        requires lowerBound(ms, bound')
+        ensures infimum(ms, val, bound) == infimum(ms, val', bound')
+    {
+    }
+    
+    lemma infimumInfSame(ms: iset<real>, val: real, bound: real, m: real)
+        requires val in ms
+        requires lowerBound(ms, bound)
+        requires inf(ms, m)
+        ensures infimum(ms, val, bound) == m
+    {
+        infAllUnique(ms, m);
+    }
+
+    ghost function supremum(ms: iset<real>, val: real, ubound: real): real
+        requires val in ms
+        requires upperBound(ms, ubound)
+        ensures sup(ms, supremum(ms, val, ubound))
+    {
+        CompletenessAxiomUpper(ms, ubound);
+        var sup_ms :| sup(ms, sup_ms);
+        sup_ms
+    }
+
+
+    lemma BoundedBelow(f: real --> real, a: real, b: real, c: real, d: real, M: real) 
+        requires M > 0.0
+        requires a < b
+        requires a <= c < d <= b
+        requires forall x :: a <= x <= b ==> f.requires(x)
+        requires isBoundedBetween(f, a, b, M)
+        ensures lowerBound(funcRange(f, c, d), -M)
+    {}
+
+    lemma BoundedAbove(f: real --> real, a: real, b: real, c: real, d: real, M: real) 
+        requires M > 0.0
+        requires a < b
+        requires a <= c < d <= b
+        requires forall x :: a <= x <= b ==> f.requires(x)
+        requires isBoundedBetween(f, a, b, M)
+        ensures upperBound(funcRange(f, c, d), M)
+    {}
+
+
+    predicate Ordered(xs: seq<real>) {
+        forall i,j :: 0 <= i < j < |xs| ==> xs[i] < xs[j]
+    }
+
+    datatype Partition = Partition(xs: seq<real>, s: set<real>)
+
+    predicate PartitionOf(a: real, b: real, p: Partition)
+        requires a < b
+    {
+        a in p.s
+        && b in p.s
+        && |p.xs| > 1
+        && (forall x :: x in p.s ==> x in p.xs)
+        && (forall x :: x in p.xs ==> x in p.s)
+        && (forall x :: x in p.xs ==> a <= x <= b)
+        && Ordered(p.xs)
+        && p.xs[0] == a
+        && p.xs[|p.xs|-1] == b
+    }
+
+    predicate PartitionPartial(a: real, b: real, p: Partition)
+        requires a < b
+    {
+        b in p.s
+        && |p.xs| > 1
+        && (forall x :: x in p.s ==> x in p.xs)
+        && (forall x :: x in p.xs ==> x in p.s)
+        && Ordered(p.xs)
+        && (forall x :: x in p.xs ==> a <= x <= b)
+        && p.xs[|p.xs|-1] == b
+    }
+
+    lemma PartitionPointsBetweenAB(p: Partition, a: real, b: real)
+        requires a < b
+        requires PartitionOf(a,b, p)
+        ensures forall x :: x in p.s ==> a <= x <= b
+    {
+    }
+
+    lemma infUnique(ms: iset<real>, m: real, m': real)
+        requires inf(ms, m)
+        requires inf(ms, m')
+        ensures m == m'
+    {
+        if m != m' {
+            assert lowerBound(ms, m);
+            assert lowerBound(ms, m');
+            if m < m' {
+                var diff := m' - m;
+                // assert diff > 0.0;
+                assert m' == add(m, diff);
+                // assert m < m+diff < m';
+                // assert lowerBound(ms, m+diff);
+                // assert !greatestLeastBound(ms, m');
+            } else {
+                var diff := m - m';
+                assert m' == add(m', diff);
+            }
+
+            assert false;
+            // assert m' <= m;
+        }
+    }
+
+    lemma infAllUnique(ms: iset<real>, m: real)
+        requires inf(ms, m)
+        ensures forall m' :: inf(ms, m') ==> m' == m
+    {
+        forall m' | inf(ms, m') 
+            ensures m' == m
+        {
+            infUnique(ms, m, m');
+        }
+    }
+
+}
